iris/TreeMove.v
@@ -954,11 +954,12 @@ Section TreeMove.
   (* ---- ...AND THE WHOLE BUNDLE, FROM ONE DEED ----------------------- *)
 
   Lemma tree_cre_commits (γfs : fs_names) (c : tree_fixed) (r : tree_names)
-      (g : gname) (t : ttree) (tyz ma mi dpar : Z) (Nm : fname -> Prop) :
+      (g : gname) (t : ttree) (tyz ma mi dpar : Z) (Nm : fname -> Prop)
+      (Nd : absnode -> Prop) :
     file_app = MkAppcfg tree_names (tree_pred c) r ->
     dpar ∈ dom (tv_nodes t) ->
     app_inv γfs -∗ tree_own r g FsImg.ROOTINO t -∗
-    cre_commits (fs_gamma_L γfs) tyz ma mi Nm (fun d : Z => ⌜d = dpar⌝%I)
+    cre_commits (fs_gamma_L γfs) tyz ma mi Nm Nd (fun d : Z => ⌜d = dpar⌝%I)
       (tree_arm_fam c r g t)
       (pfam_triv (fun _ _ _ _ => True%I))
       (tree_unarm_fam c r g t)
@@ -974,6 +975,8 @@ Section TreeMove.
       iApply (tree_dots_commit γfs c r Heq). }
     iSplitR.
     { rewrite /pf_at. iSplit; [| cbn [pf_refund]; done].
+      iApply (aunarm_of_arm_nd_of (fs_gamma_L γfs) appE Nd
+                (tree_arm_fam c r g t) _).
       iApply (tree_unarm_commit γfs c r g t Heq with "Hinv"). }
     rewrite /pf_at. iSplit; [| cbn [pf_refund]; done].
     (* a provider that answers at EVERY name answers at the ones [Nm]
@@ -1039,11 +1042,17 @@ Section TreeMove.
         iApply pf_at_triv. iApply dlookup_commit_at_unit. }
       (* THE CHILD'S TWO LEGS: the deed goes in HERE and comes back out in
          the arm's receipt *)
-      rewrite /cre_child_unfired. iSplitL "Hown".
+      rewrite /cre_child_unfired_nd. iSplitL "Hown".
       - rewrite /pf_at /tree_arm_fam /=. iSplit; [| iExact "Hown"].
         iApply (tree_arm_commit γfs c r g t (ADev ma mi) Heq
                   (tabs_leaf_dev ma mi) with "Hinv Hown").
       - rewrite /pf_at /tree_unarm_fam /=. iSplit; [| done].
+        (* the unarm at the node sys_mknod PINS: a provider that answers at
+           EVERY node answers at that one
+           ([FsAbsCreateNm.aunarm_of_arm_nd_of]) *)
+        iApply (aunarm_of_arm_nd_of (fs_gamma_L γfs) appE
+                  (fun c' : absnode => c' = ADev ma mi)
+                  (tree_arm_fam c r g t) _).
         iApply (tree_unarm_commit γfs c r g t Heq with "Hinv"). }
     (* THE PARENT LEG, at the guarded cursor: the move between the two
        readings is the ISO, and it costs nothing because the cursor is
@@ -1176,7 +1185,7 @@ Section TreeMove.
       - iApply (ep_hops_done γfs _ _ pl 0%nat). rewrite Hnp /=. lia. }
     iSplitR.
     { iApply pf_at_triv. iApply dlookup_commit_at_unit. }
-    iApply (cre_commits_mono (fs_gamma_L γfs) _ _ _ _
+    iApply (cre_commits_mono (fs_gamma_L γfs) _ _ _ _ _
               (fun d : Z => ⌜d = FsImg.ROOTINO⌝%I)
               (npar_cur M pv (fun (_ : nat) (d : Z) => ⌜d = FsImg.ROOTINO⌝%I))
               with "[] [] [Hown]").
@@ -1184,7 +1193,7 @@ Section TreeMove.
       iApply ("H" $! pl). iPureIntro. exact Hpath.
     - iIntros "!>" (d) "%Hd". rewrite /npar_cur. iIntros (pl0) "_".
       by iPureIntro.
-    - iApply (tree_cre_commits γfs c r g t _ _ _ FsImg.ROOTINO _ Heq Hdd
+    - iApply (tree_cre_commits γfs c r g t _ _ _ FsImg.ROOTINO _ _ Heq Hdd
                 with "Hinv Hown").
   Qed.
 
